sequences.v
@@ -1,0 +1,133 @@
+From networks Require Import listidx.
+
+Set Implicit Arguments.
+
+Section sequences.
+    
+
+CoInductive seq (A:Type) : Type := 
+  | nil : seq A
+  | cons : A -> seq A -> seq A
+.
+ 
+Arguments nil {A}. 
+
+Inductive  isinIndex {A:Type} : seq A -> nat ->  Prop :=
+    | IO : forall a s, isinIndex (cons a s) O
+    | IN : forall a s n,  isinIndex s n ->  isinIndex (cons a s) (S n)
+. 
+
+
+Lemma nil_impossible {A:Type} (n:nat) :  ~isinIndex (A:=A) nil n.
+Proof.
+    unfold "~". intros. inversion H. 
+Qed.
+
+Lemma step_back {A:Type} (a:A) (s:seq A) (n: nat)  : isinIndex (cons a s) (S n) -> isinIndex s n.
+Proof.
+    intros.  inversion H. exact H1. 
+Qed.
+
+Lemma switch {A:Type} (a0 a1:A) (s:seq A) (n: nat) : isinIndex (cons a0  (cons a1 s)) n -> isinIndex (cons a1  (cons a0 s)) n.
+Proof.
+    intros.  induction n.  apply IO.  apply step_back in H. induction n. apply IN. apply IO. apply step_back in H. 
+    apply (IN a1 (IN a0 H)).
+Qed.
+
+
+Theorem add_one (A:Type) (s:seq A) (n: nat) (a:A) : isinIndex s n  -> isinIndex (cons a s) n.
+Proof.
+    intros. induction H. apply IO. apply (IN a0) in IHisinIndex. apply (switch IHisinIndex).
+Qed.
+
+Theorem skip_one (A:Type) (s:seq A) (n: nat) : isinIndex s (S n ) -> isinIndex s n.
+Proof.
+    intros. destruct s. apply nil_impossible in H. contradiction. apply step_back in H. apply (add_one a) in H. apply H.
+Qed.
+
+
+
+
+Definition indexOf {A:Type} (s:seq A)  := { n:nat | isinIndex s n}.
+Definition index  {A:Type} {l:seq A} (i:indexOf l) := proj1_sig i.
+Definition rangeproof  {A:Type} {l:seq A} (i:indexOf l) := proj2_sig i.
+Definition mkIndex {A:Type} (l:seq A) (n:nat) (p:isinIndex l n) : indexOf l := (exist (fun x => isinIndex l x) n p).
+(* Coercion index : indexOf >-> nat. *)
+
+
+Definition makeSig (A : Type) (P : A -> Prop) (x : A) (p : P x) : sig P :=
+    exist P x p.
+#[global]Arguments makeSig [A]%type_scope [P]%function_scope [x] p.
+
+
+(* 
+Definition destructIndex {A:Type} {s:seq A} (i:indexOf s) :  
+    (index i = 0) + (exists (a:A) (n:nat) (p:isinIndex (cons a s) (S n)), (index i = S n)).
+Proof.
+    destruct i. simpl. destruct x. auto. right.  destruct s. apply nil_impossible in i. contradiction.
+    exists a. exists x.  *)
+     
+
+
+Theorem absurd_type : forall (A:Prop) (C:Type), A -> ~ A -> C.
+Proof.
+  intros A C h1 h2.
+  apply False_rect.
+  apply (h2 h1).
+Qed.
+
+Fixpoint trim_unpacked {A:Type} (s:seq A) (n: nat)  : isinIndex s n -> (A * seq A) := 
+    match s, n return  isinIndex s n ->  (A * seq A) with
+        | nil,_           => fun h : isinIndex nil n              => absurd_type _ h (nil_impossible (n:=n))
+        | cons a s', S n' => fun h : isinIndex (cons a s') (S n') => trim_unpacked (step_back h)
+        | cons a s', 0    => fun _                                =>  pair a s'
+    end.
+
+Definition trim {A:Type} (s:seq A) (i:indexOf s) : (A * seq A) := 
+    trim_unpacked (rangeproof i)
+.
+
+Fixpoint elem_unpacked {A:Type} (s:seq A) (n: nat)  : isinIndex s n -> A := 
+    match s, n return  isinIndex s n ->  A with
+        | nil,_ => fun h : isinIndex nil n  => absurd_type A h (nil_impossible (n:=n))
+        | cons a s', S n' => fun h :  isinIndex (cons a s') (S n') => elem_unpacked (step_back h)
+        | cons a s', 0 => fun h :  isinIndex (cons a s') 0 =>  a
+    end.
+
+Definition elem {A:Type} (s:seq A) (i:indexOf s) : A := 
+    elem_unpacked (rangeproof i)
+.
+
+
+Fixpoint tail_unpacked {A:Type} (s:seq A) (n: nat)  : isinIndex s n -> seq A := 
+    match s, n return  isinIndex s n -> seq A with
+        | nil,_           => fun h : isinIndex nil n  => absurd_type (seq A) h (nil_impossible (n:=n))
+        | cons a s', S n' => fun h :  isinIndex (cons a s') (S n') => tail_unpacked (step_back h)
+        | cons a s', 0    => fun h :  isinIndex (cons a s') 0 =>  s'
+    end.
+
+Definition tail {A:Type} (s:seq A) (i:indexOf s) : seq A := 
+    tail_unpacked (rangeproof i)
+.
+
+CoFixpoint map {A B:Type} (s:seq A) (f: A->B) : seq B :=
+    match s with
+      | nil => nil
+      | cons a t => cons (f a)  (map t f)
+    end.
+
+
+Inductive isPrefixOf {A:Type}  : list A  -> seq A -> Prop :=
+    | prefixN : forall a l s, isPrefixOf l s -> isPrefixOf (List.cons a l) (cons a s)
+    | prefixO : isPrefixOf List.nil nil
+.
+
+Fixpoint asSeq (A:Type) (l : list A) : seq A := 
+    match l with
+        | List.cons a l' => cons a (asSeq l')
+        | List.nil => nil
+    end.
+
+Definition subseq {A:Type} (s:seq A) (P: A -> Prop) := { i:indexOf s | P (elem i)}.
+
+End sequences.
