README.md
@@ -1,2 +1,4 @@
 # network_models
 This is an experimental formalisation of the network model introduced in [my thesis](https://tel.archives-ouvertes.fr/tel-03583890/document).
+
+This project is a learning ground, questionable code lies ahead.
